src/Init/Data/String/Extra.lean
@@ -32,21 +32,26 @@ theorem one_le_csize (c : Char) : 1 ≤ csize c := by
   simp [csize, Char.utf8Size]
   repeat (first | split | decide)
 
-theorem eq_empty_of_bsize_eq_zero (h : s.bsize = 0) : s = "" := by
+@[simp] theorem pos_lt_eq (p₁ p₂ : Pos) : (p₁ < p₂) = (p₁.1 < p₂.1) := rfl
+
+@[simp] theorem pos_add_char (p : Pos) (c : Char) : (p + c).byteIdx = p.byteIdx + csize c := rfl
+
+theorem eq_empty_of_bsize_eq_zero (h : s.endPos = {}) : s = "" := by
   match s with
   | ⟨[]⟩   => rfl
   | ⟨c::cs⟩ =>
-    simp [bsize, utf8ByteSize, utf8ByteSize.go] at h
+    injection h with h
+    simp [endPos, utf8ByteSize, utf8ByteSize.go] at h
     have : utf8ByteSize.go cs + 1 ≤ utf8ByteSize.go cs + csize c := Nat.add_le_add_left (one_le_csize c) _
     simp_arith [h] at this
 
-theorem lt_next (s : String) (i : String.Pos) : i < s.next i := by
+theorem lt_next (s : String) (i : String.Pos) : i.1 < (s.next i).1 := by
   simp_arith [next]; apply one_le_csize
 
 theorem Iterator.sizeOf_next_lt (i : String.Iterator) (h : i.hasNext) : sizeOf i.next < sizeOf i := by
   cases i; rename_i s pos; simp [Iterator.next, Iterator.sizeOf_eq]; simp [Iterator.hasNext] at h
   have := String.lt_next s pos
-  apply Nat.sub.elim (motive := fun k => k < _) (utf8ByteSize s) (String.next s pos)
+  apply Nat.sub.elim (motive := fun k => k < _) (utf8ByteSize s) (String.next s pos).1
   . intro hle k he
     simp [he]; rw [Nat.add_comm, Nat.add_sub_assoc (Nat.le_of_lt this)]
     have := Nat.zero_lt_sub_of_lt this
